messageInvariantPrototypes/ringLeaderElection/decentralizedMonotonic/messageInvariants.dfy
@@ -1,0 +1,135 @@
+// Network-level "boilerplate" invariants that are application-independent
+
+include "spec.dfy"
+
+module MessageInvariants {
+import opened Types
+import opened UtilitiesLibrary
+import opened DistributedSystem
+import opened Obligations
+
+// All msg have a valid ringPos as src
+ghost predicate VoteMsgValidSrc(c: Constants, v: Variables)
+  requires v.WF(c)
+{
+  forall msg | msg in v.network.sentMsgs
+  :: c.ValidIdx(msg.src)
+}
+
+// Every message is sent according to a fixed function
+ghost predicate TransmissionValidity(c: Constants, v: Variables)
+  requires v.WF(c)
+  requires VoteMsgValidSrc(c, v)
+{
+  forall msg | msg in v.network.sentMsgs
+  :: 
+  (exists i, src ::
+      && v.ValidHistoryIdx(i)
+      && c.ValidIdx(src)
+      && msg == Msg(max(v.History(i).hosts[src].highestHeard, c.hostConstants[src].hostId), src)
+  )
+}
+
+// For each host, if its highestHeard is >-1, then it must have gotten it from a message
+// from its predecessor
+ghost predicate ReceiveValidity(c: Constants, v: Variables) 
+  requires v.WF(c)
+{
+  forall i, idx | 
+    && v.ValidHistoryIdx(i)
+    && c.ValidIdx(idx)
+    && v.History(i).hosts[idx].highestHeard > -1
+  :: 
+    (exists msg :: 
+        && msg in v.network.sentMsgs 
+        && msg.src < c.hostConstants[idx].numParticipants
+        && idx == Successor(c.hostConstants[idx].numParticipants, msg.src)
+        // && v.History(i).hosts[idx].highestHeard < msg.val
+        && msg.val == v.History(i).hosts[idx].highestHeard 
+    )
+}
+
+ghost predicate MessageInv(c: Constants, v: Variables)
+{
+  && v.WF(c)
+  && VoteMsgValidSrc(c, v)
+  && TransmissionValidity(c, v)
+  && ReceiveValidity(c, v)
+}
+
+lemma InitImpliesMessageInv(c: Constants, v: Variables)
+  requires Init(c, v)
+  ensures MessageInv(c, v)
+{}
+
+lemma MessageInvInductive(c: Constants, v: Variables, v': Variables)
+  requires MessageInv(c, v)
+  requires Next(c, v, v')
+  ensures MessageInv(c, v')
+{
+  InvNextTransmissionValidity(c, v, v');
+  InvNextReceiveValidity(c, v, v');
+}
+
+
+/***************************************************************************************
+*                                         Proofs                                       *
+***************************************************************************************/
+
+lemma InvNextTransmissionValidity(c: Constants, v: Variables, v': Variables)
+  requires v.WF(c)
+  requires VoteMsgValidSrc(c, v)
+  requires TransmissionValidity(c, v)
+  requires Next(c, v, v')
+  ensures TransmissionValidity(c, v')
+{
+  VariableNextProperties(c, v, v');
+}
+
+lemma InvNextReceiveValidity(c: Constants, v: Variables, v': Variables)
+  requires v.WF(c)
+  requires ReceiveValidity(c, v)
+  requires Next(c, v, v')
+  ensures ReceiveValidity(c, v')
+{
+  VariableNextProperties(c, v, v');
+  forall i, idx | 
+    && v'.ValidHistoryIdx(i)
+    && c.ValidIdx(idx)
+    && v'.History(i).hosts[idx].highestHeard > -1
+  ensures
+    (exists msg :: 
+        && msg in v'.network.sentMsgs 
+        && msg.src < c.hostConstants[idx].numParticipants
+        && idx == Successor(c.hostConstants[idx].numParticipants, msg.src)
+        // && v'.History(i).hosts[idx].highestHeard < msg.val
+        && msg.val == v'.History(i).hosts[idx].highestHeard 
+    )
+  {
+    if i == |v'.history|-1 {
+      var dsStep :| NextStep(c, v.Last(), v'.Last(), v.network, v'.network, dsStep);
+      var h, h', actor, msgOps := v.Last(), v'.Last(), dsStep.actorIdx, dsStep.msgOps;
+      assert Host.Next(c.hostConstants[actor], h.hosts[actor], h'.hosts[actor], msgOps);
+      var cs, s, s' := c.hostConstants[actor], h.hosts[actor], h'.hosts[actor];
+      var step :| Host.NextStep(cs, s, s', step, msgOps);
+      if step.ReceiveStep? {
+        var msg := msgOps.recv.value;
+      }
+    }
+  }
+}
+
+
+lemma VariableNextProperties(c: Constants, v: Variables, v': Variables)
+  requires v.WF(c)
+  requires Next(c, v, v')
+  ensures 1 < |v'.history|
+  ensures |v.history| == |v'.history| - 1
+  ensures v.Last() == v.History(|v'.history|-2) == v'.History(|v'.history|-2)
+  ensures forall i | 0 <= i < |v'.history|-1 :: v.History(i) == v'.History(i)
+{
+  assert 0 < |v.history|;
+  assert 1 < |v'.history|;
+}
+} // end module MessageInvariants
+
